src/HOL/Hoare_Parallel/Quote_Antiquote.thy
@@ -6,13 +6,10 @@ theory Quote_Antiquote imports Main begin
 syntax
   "_quote"     :: "'b \<Rightarrow> ('a \<Rightarrow> 'b)"                ("(\<guillemotleft>_\<guillemotright>)" [0] 1000)
   "_antiquote" :: "('a \<Rightarrow> 'b) \<Rightarrow> 'b"                ("\<acute>_" [1000] 1000)
-  "_Assert"    :: "'a \<Rightarrow> 'a set"                    ("(.{_}.)" [0] 1000)
-
-syntax (xsymbols)
-  "_Assert"    :: "'a \<Rightarrow> 'a set"            ("(\<lbrace>_\<rbrace>)" [0] 1000)
+  "_Assert"    :: "'a \<Rightarrow> 'a set"                    ("(\<lbrace>_\<rbrace>)" [0] 1000)
 
 translations
-  ".{b}." \<rightharpoonup> "CONST Collect \<guillemotleft>b\<guillemotright>"
+  "\<lbrace>b\<rbrace>" \<rightharpoonup> "CONST Collect \<guillemotleft>b\<guillemotright>"
 
 parse_translation {*
   let
